start setting up a representation invariant for malloc

theories/iris/allocator/function/malloc.v
@@ -22,26 +22,53 @@ Section malloc.
 Section code.
   
 (*
+enum state_t ::= FREE | USED | STOP
 
-[ free? ][ size ] [ next ] .....  [ free? ] [ size ] [ next ] ...
+struct block {
+  state_t   state;
+  // rest of this is only present if state != STOP
+  i32       size; // must be nonzero
+  i32       next;
+  i32[size] data;
+}
+[ state ][ size ][ next ] .....  [ state ][ size ][ next ] ...
 
 *)
+  
+Definition BLK_FREE : N := 0.
+Definition BLK_USED : N := 1.
+Definition BLK_STOP : N := 2.
 
-(* Given a pointer to a block in the free list, return the block's free flag. *)
-Definition get_block_free :=
+(* Given a pointer to a block in the free list, return the block's state marker. *)
+Definition get_block_state :=
   [
     BI_load T_i32 None 0%N 0%N
   ].
 
+Definition get_block_stop := 
+  get_block_state ++
+  [u32const BLK_STOP;
+   BI_relop T_i32 (Relop_i ROI_eq)].
+
+Definition get_block_free := 
+  get_block_state ++
+  [u32const BLK_FREE;
+   BI_relop T_i32 (Relop_i ROI_eq)].
+
+Definition get_block_used := 
+  get_block_state ++
+  [u32const BLK_USED;
+   BI_relop T_i32 (Relop_i ROI_eq)].
+
 Definition mark_block_free :=
   [
-    i32const 1;
+    u32const BLK_FREE;
     BI_store T_i32 None 0%N 0%N
   ].
 
 Definition mark_block_used :=
   [
-    i32const 0;
+    u32const BLK_USED;
     BI_store T_i32 None 0%N 0%N
   ].
 
@@ -84,9 +111,12 @@ Definition malloc :=
     (* Store the current block in $1. *)
     BI_set_local 1
   ] ++ [
-    BI_loop (Tf [] []) [
+    (* Loop invariant: $1 is either -1 or it points to a valid block. *)
+    BI_loop (Tf [] []) (
+      (* Check if the block is a STOP marker. *)
+      BI_get_local 1 ::
+      get_block_stop ++ [
       BI_if (Tf [] [])
-          (* address of block was non-null: check free flag and size *)
           (* put the free flag at the top of the stack*)
           (BI_get_local 1 ::
            get_block_free ++
@@ -106,50 +136,140 @@ Definition malloc :=
                 [BI_return]
             ) 
             (get_block_next ++ [BI_set_local 1])
-      ]) [
+          ]) [
           (* address of block was null: trap *)
           (* grow the free list *)
           (* ultimately, decide we're out of space & return -1 *)
           BI_unreachable
       ]
-    ]
+    ]) 
   ].
 
 End code.
 
 Section specs.
 
-Lemma spec_malloc E free_flag next_ptr f0 sz: 
-  ⊢ {{{{ ⌜ f0.(f_inst).(inst_memory) !! 0 = Some free_flag⌝ ∗
-         ⌜ f0.(f_inst).(inst_memory) !! 4 = Some next_ptr ⌝ ∗
-         ⌜ f0.(f_locs) !! 0 = Some sz⌝ ∗
-         ⌜ length (f_locs f0) >= 2 ⌝ ∗
-        ↪[frame] f0
+Lemma wp_label_push_emp
+  (s : stuckness) (E : coPset) (Φ : val → iProp Σ)
+  (es : language.expr iris_wp_def.wasm_lang) 
+  (i : nat) (lh : lholed) (n : nat) 
+  (es' : seq.seq administrative_instruction) :
+  WP es @ s; E CTX S i; push_base lh n es' [] [] {{ v, Φ v }} ⊢ WP [AI_label n es' es] @ s; E CTX i; lh {{ v, Φ v }}.
+Proof.
+  replace [AI_label n es' es] 
+     with [AI_label n es' ([] ++ es ++ [])]
+    by (rewrite cats0; auto).
+  eapply wp_label_push; auto.
+Qed.
+
+Lemma wp_label_push_cons
+  (s : stuckness) (E : coPset) (Φ : val → iProp Σ)
+  (e : administrative_instruction)
+  (es : language.expr iris_wp_def.wasm_lang) 
+  (i : nat) (lh : lholed) (n : nat) 
+  (es' : seq.seq administrative_instruction) :
+  WP [e] @ s; E CTX S i; push_base lh n es' [] es {{ v, Φ v }} ⊢ WP [AI_label n es' (e::es)] @ s; E CTX i; lh {{ v, Φ v }}.
+Proof.
+  replace [AI_label n es' (e::es)] 
+     with [AI_label n es' ([] ++ [e] ++ es)]
+    by (simpl; auto).
+  eapply wp_label_push; auto.
+Qed.
+
+Inductive free_flag :=
+| Used
+| Free.
+
+Definition flag_repr (flag : free_flag) : value :=
+  match flag with
+  | Used => value_of_uint BLK_USED
+  | Free => value_of_uint BLK_FREE
+  end.
+
+Inductive block :=
+| BlkStop: block
+| BlkGo: 
+  free_flag -> 
+  i32 (* size *) ->
+  block (* next *) ->
+  block.
+
+Definition nat_repr (n: nat) (m: i32) : Prop :=
+  Z.of_nat n = Wasm_int.Int32.unsigned m.
+
+Definition own_block (memidx: N) (base_addr: N) (sz: i32) : iProp Σ :=
+  ∃ bs: bytes, ⌜nat_repr (length bs) sz⌝ ∗ memidx ↦[wms][base_addr] bs.
+
+Definition data_repr (flag: free_flag) (sz: i32) (memidx: N) (base_addr: N) : iProp Σ :=
+  match flag with
+  | Used => ⌜True⌝
+  | Free => own_block memidx base_addr sz
+  end%I.
+
+(* The block representation invariant *)
+Fixpoint blk_rep blk memidx base_addr : iProp Σ :=
+  match blk with
+  | BlkStop =>
+      memidx ↦[wms][base_addr] bits (value_of_uint BLK_STOP)
+  | BlkGo flag sz next =>
+      ∃ next_addr,
+        memidx ↦[wms][base_addr] bits (flag_repr flag) ∗
+        memidx ↦[wms][base_addr + 4] bits (VAL_int32 sz) ∗
+        memidx ↦[wms][base_addr + 8] bits (value_of_uint next_addr) ∗
+        data_repr flag sz memidx (base_addr + 12)%N ∗
+        blk_rep next memidx next_addr
+  end%I.
+
+Lemma spec_malloc E f0 reqd_sz (memidx: memaddr) blk :
+  ⊢ {{{{ ⌜f0.(f_inst).(inst_memory) !! 0 = Some memidx⌝ ∗
+         ⌜f0.(f_locs) !! 0 = Some (VAL_int32 reqd_sz)⌝ ∗
+         ⌜length (f_locs f0) >= 2⌝ ∗
+         blk_rep blk (N.of_nat memidx) 0 ∗
+         ↪[frame] f0
     }}}}
     (to_e_list malloc) @ E
-    {{{{ v, ⌜True⌝ }}}}.
+    {{{{ v, ∃ ret_addr, ⌜v = immV [value_of_uint ret_addr]⌝ ∗
+            ∃ blk', blk_rep blk' (N.of_nat memidx) 0 ∗ 
+                    own_block (N.of_nat memidx) ret_addr reqd_sz ∗
+                    ↪[frame] f0 }}}}.
 Proof.
-  iIntros "!>" (Φ) "(%Hfree & %Hnext & %Hsz & %Hlen & Hfr) HΦ".
+  iIntros "!>" (Φ) "(%Hmemidx & %Hsz & %Hlen & Hblk & Hfr) HΦ".
   unfold malloc.
   erewrite !to_e_list_cat.
+  set (f1 := {| f_locs := set_nth (value_of_uint 0) (f_locs f0) 1 (value_of_uint 0);
+                f_inst := f_inst f0 |}).
   iApply wp_seq.
-  instantiate (1 := λ v, (⌜v = immV []⌝ ∗
-                         ↪[frame] {|
-                           f_locs := set_nth (value_of_uint 0) (f_locs f0) 1 (value_of_uint 0);
-                           f_inst := f_inst f0 |})%I).
+  instantiate (1 := λ v, (⌜v = immV []⌝ ∗ ↪[frame] f1)%I).
   iSplitR.
   { iIntros "(%Htrap & _)". auto. }
   iSplitL "Hfr".
-  { cbn. 
+  {
+    cbn. 
     unfold i32const.
     iApply wp_set_local => //.
   }
   iIntros (w) "(%Htrap & Hfr)".
   subst w.
-
-  iApply (wp_loop with "[Hfr] [HΦ]") => //; eauto.
+  iApply wp_wasm_empty_ctx.
+  iApply (wp_loop_ctx with "[Hfr] [HΦ]") => //; eauto.
   iIntros "!> Hfr".
-  (* unsure what to do here. *)
+  iApply wp_label_push_emp.
+  iApply wp_ctx_bind; [cbn; tauto|].
+  cbn.
+  take_drop_app_rewrite 1.
+  iApply wp_seq; cbn.
+  instantiate (1 := λ v, (⌜v = immV [value_of_uint 0]⌝ ∗ ↪[frame] f1)%I).
+  iSplitR.
+  { iIntros "(%Htrap & _)" => //. }
+  iSplitL "Hfr".
+  { 
+    iApply wp_get_local => //.
+    apply set_nth_read.
+  }
+  iIntros (w) "(%Hzero & Hfr)".
+  subst w.
+  take_drop_app_rewrite 2.
+  iApply wp_seq; cbn.
 Admitted.
 
 End specs.    
